\subsection{}

Describe the evaluation of the following terms:
\begin{enumerate}
\item $M_1 = \FST{\PAIR{\SUM{4}{1}}{\IF{true}{false}{false}}}$:
  \[
  \infer[\text{\small{(project-1)}}]
	{ \FST{\PAIR{\SUM{4}{1}}{\IF{true}{false}{false}}} \to \FST{\PAIR{5}{\IF{true}{false}{false}}}}
	{
	  \infer[\text{\small{(eval-pair 1)}}]
		{ \PAIR{\SUM{4}{1}}{\IF{true}{false}{false}} \to \PAIR{5}{\IF{true}{false}{false}} }
		{ \infer[\text{\small{(sum)}}]{\SUM{4}{1} \to 5}{} }
	}
	\]
	\[
	\infer[\text{\small{(project-1)}}]
	      { \FST{\PAIR{5}{\IF{true}{false}{false}}} \to \FST{\PAIR{5}{false}}}
	      {
		\infer[\text{\small{(eval-pair 2)}}]
		      { \PAIR{5}{\IF{true}{false}{false}} \to \PAIR{5}{false}}
		      { \infer[\text{\small(if-true)}]{\IF{true}{false}{false} \to false}{} }
	      }
	      \]
	      \[
	      \infer[\text{\small{(pair 1)}}]
		    { \FST{\PAIR{5}{false}} \to 5}{}
	            \]
	          \item $M_2 = \APP{(\FN{x: Nat \ast Nat}{\SND{x}})}{\PAIR{\SUM{4}{2}}{\SUM{3}{1}}}$:
	            \[
		    \infer[\text{\small{(app-2)}}]
		          {\APP{(\FN{x: Nat \ast Nat}{\SND{x}})}{\PAIR{\SUM{4}{2}}{\SUM{3}{1}}} \to \APP{(\FN{x: Nat \ast Nat}{\SND{x}})}{\PAIR{6}{\SUM{3}{1}}}}
		          {
			    \infer[\text{\small{(eval-pair 1)}}]
			          {\PAIR{\SUM{4}{2}}{\SUM{3}{1}} \to \PAIR{6}{\SUM{3}{1}}}
			          {
				    \infer[\text{\small{(sum)}}]{\SUM{4}{2} \to 6}{}
			          }
		          }
	                  \]
	                  \[
		          \infer[\text{\small{(app-2)}}]
		                {\APP{(\FN{x: Nat \ast Nat}{\SND{x}})}{\PAIR{6}{\SUM{3}{1}}} \to \APP{(\FN{x: Nat \ast Nat}{\SND{x}})}{\PAIR{6}{4}}}
		                {
			          \infer[\text{\small{(eval-pair 2)}}]
			                {\PAIR{6}{\SUM{3}{1}} \to \PAIR{6}{4}}
			                { \infer[\text{\small{(sum)}}]{\SUM{3}{1} \to 4}{} }
		                }
	                        \]
	                        \[
		                \infer[\text{\small{(beta)}}]
		                      {\APP{(\FN{x: Nat \ast Nat}{\SND{x}})}{\PAIR{6}{4}} \to \SND{\PAIR{6}{4}}}
		                      {}
	                              \]
	                              \[
		                      \infer[\text{\small{(pair 2)}}]{\SND{\PAIR{6}{4}} \to 4}{}
	                              \]
	                            \item $M_3 = \SND{(\SUM{(\SUM{3}{2})}{1})}$:
	                              \[
		                      \infer[\text{\small{(project-2)}}]
		                            {\SND{(\SUM{(\SUM{3}{2})}{1})} \to \SND{(\SUM{5}{1})}}
		                            {
			                      \infer[\text{\small{(sum-l)}}]
			                            {\SUM{(\SUM{3}{2})}{1} \to \SUM{5}{1}}
			                            {
				                      \infer[\text{\small{(sum)}}]{\SUM{3}{2} \to 5}{}
			                            }
		                            }
	                                    \]
	                                    \[
		                            \infer[\text{\small{(project-2)}}]
		                                  {\SND{(\SUM{5}{1})} \to \SND{(6)}}
		                                  { \infer[\text{\small{(sum)}}]{\SUM{5}{1} \to 6}{} }
	                                          \]
	                                          \[
		                                  \infer{\SND{(6)} \not\to }{}
	                                          \]
\end{enumerate}
