\subsection{}

Think of a possible Strengthening Lemma which, in contrast to the Weakening
Lemma, strengthens the contextual assumptions.

If $\Gamma, x: T' \vdash M: T$ is a derivable judgement and $x \notin \fv{M}$ then
$\Gamma \vdash M: T$ is derivable.\\
The proof will proceed by induction on the derivation tree of the judgement
$\Gamma, x: T' \vdash M: T$:

\paragraph*{Base cases: $h = 1$:\\}

The base cases are those where the last typing rule is an axiom:
\begin{itemize}
	\item (T-TRUE):
	      if $\Gamma, x: T' \vdash true: Bool$ is derivable and
	      $x \notin \fv{true} = \emptyset$, $\Gamma \vdash true: Bool$ derivable by T-TRUE typing rule
	\item (T-FALSE):
	      if $\Gamma, x: T' \vdash false: Bool$ is derivable and
	      $x \notin \fv{false} = \emptyset$, $\Gamma \vdash false: Bool$ derivable by T-FALSE typing rule
	\item (T-INT):
	      if $\Gamma, x: T' \vdash n: Nat$ is derivable and
	      $x \notin \fv{n} = \emptyset$, $\Gamma \vdash n: Nat$ derivable by T-INT typing rule
	\item (T-VAR):
	      if $\Gamma, x: T' \vdash y: T$ is derivable and
	      $x \notin \fv{y} = \{y\}$, then $x \ne y$ hence
	      $y \in Dom(\Gamma) \subseteq Dom(\Gamma, x: T')$ thus $\Gamma \vdash y: T$ derivable by
	      T-VAR typing rule
\end{itemize}

\paragraph*{Inductive cases: $h = h_0 + 1$:\\}

The inductive hypothesis is that for any derivable judgement\\
$\Gamma, x: T' \vdash M: T$ of height $h \le h_0$ if $x \notin \fv{M}$ then $\Gamma \vdash M: T$.
The inductive cases will be distinguished based on the last typing rule applied to the
derivation tree:
\begin{itemize}
	\item (T-SUM): $M = \SUM{M_1}{M_2}$
	      if $\Gamma, x: T' \vdash M: T$ is derivable and $x \notin \fv{M} = \fv{M_1}\cup\fv{M_2}$,
	      then $x \notin \fv{M_1}, \fv{M_2}$ and by Inversion Lemma:
	      \begin{itemize}
		      \item $\Gamma, x: T' \vdash M_1 : Nat$ derivable
		      \item $\Gamma, x: T' \vdash M_2 : Nat$ derivable
	      \end{itemize}
	      and since their derivation trees have height $h_0$ the inductive hypothesis can be applied;
	      hence
	      \begin{itemize}
		      \item $\Gamma \vdash M_1 : Nat$ derivable
		      \item $\Gamma \vdash M_2 : Nat$ derivable
	      \end{itemize}
	      Thus by T-SUM rule $\Gamma \vdash M: T$ is derivable
	\item (T-IFTHENELSE): $M = \IF{M_1}{M_2}{M_3}$
	      if $\Gamma, x: T' \vdash M: T$ is derivable and
	      $x \notin \fv{M} = \fv{M_1}\cup\fv{M_2}\cup\fv{M_3}$, then
	      $x \notin \fv{M_1}, \fv{M_2}, \fv{M_3}$ and by Inversion Lemma:
	      \begin{itemize}
		      \item $\Gamma, x: T' \vdash M_1 : Bool$ derivable
		      \item $\Gamma, x: T' \vdash M_2 : T$ derivable
		      \item $\Gamma, x: T' \vdash M_2 : T$ derivable
	      \end{itemize}
	      and since their derivation trees have height $h_0$ the inductive hypothesis can be applied;
	      hence
	      \begin{itemize}
		      \item $\Gamma \vdash M_1 : Bool$ derivable
		      \item $\Gamma \vdash M_2 : T$ derivable
		      \item $\Gamma \vdash M_2 : T$ derivable
	      \end{itemize}
	      Thus by T-IF rule $\Gamma \vdash M: T$ is derivable
	\item (T-FUN): $M = \FN{y: T_1}{M_1}$
	      if $\Gamma, x: T' \vdash M: T$ is derivable and $x \notin \fv{M} = \fv{M_1}\setminus\{x\}$.
	      (In case that $y = x$ it can be chosen an $\alpha$-equivalent term
	      $\FN{y: T_1}{M_1} =_{\alpha} \FN{z: T_1}{M_1\SUBST{y}{z}}$ such that
	      $z \notin Dom(\Gamma,x: T')$)\\
	      Then $x \notin \fv{M_1}$ and by Inversion Lemma $\exists\, T_2$ such that:
	      \begin{itemize}
		      \item $T= T_1 \to T_2$
		      \item $\Gamma, x: T', y: T_1 \vdash M_1: T_2$ derivable
	      \end{itemize}
	      and since it's derivation tree has height $h_0$ the inductive hypothesis can be applied;
	      hence\\ $\Gamma, y: T_1 \vdash M_1: T_2$ derivable, thus by T-FUN rule
	      $\Gamma \vdash M: T$ derivable
	\item (T-APP): $M = \APP{M_1}{M_2}$
	      if $\Gamma, x: T' \vdash M: T$ is derivable and $x \notin \fv{M} = \fv{M_1}\cup\fv{M_2}$,
	      then $x \notin \fv{M_1}, \fv{M_2}$ and by Inversion Lemma $\exists\, T_1$ such that:
	      \begin{itemize}
		      \item $\Gamma, x: T' \vdash M_1 : T_1 \to T$ derivable
		      \item $\Gamma, x: T' \vdash M_2 : T_1$ derivable
	      \end{itemize}
	      and since their derivation trees have height $h_0$ the inductive hypothesis can be applied;
	      hence
	      \begin{itemize}
		      \item $\Gamma \vdash M_1 : T_1 \to T$ derivable
		      \item $\Gamma \vdash M_2 : T$ derivable
	      \end{itemize}
	      Thus by T-APP rule $\Gamma \vdash M: T$ is derivable
\end{itemize}














