\subsection{}

Show the evaluation of the term
$\APP{(\APP{(\FN{x}{3})}{(\FN{y}{y})})}{(\APP{(\FN{z}{\IF{z}{1}{0}})}{(false)})}$.
Define a variant of the evaluation rules so that, by keeping a call-by-value
strategy, the previous term evolves to a stuck term in fewer reduction steps.
\[
	\infer[\text{\small{APP 1}}]
	{
		\APP{(\APP{(\FN{x}{3})}{(\FN{y}{y})})}{(\APP{(\FN{z}{\IF{z}{1}{0}})}{(false)})} \to
		\APP{3}{(\APP{(\FN{z}{\IF{z}{1}{0}})}{(false)})}
	}
	{
		\infer[\text{\small{BETA}}]
		{
			\APP{(\FN{x}{3})}{(\FN{y}{y})} \to 3
		}
		{}
	}
\]
\\
\[
	\infer[\text{\small{APP 2}}]
	{
		\APP{3}{(\APP{(\FN{z}{\IF{z}{1}{0}})}{(false)})} \to
		\APP{3}{(\IF{false}{1}{0})}
	}
	{
		\infer[\text{\small{BETA}}]
		{
			\APP{(\FN{z}{\IF{z}{1}{0}})}{(false)} \to \IF{false}{1}{0}
		}
		{}
	}
\]
\\
\[
	\infer[\text{\small{APP 2}}]
	{
		\APP{3}{(\IF{false}{1}{0})} \to
		\APP{3}{0}
	}
	{
		\infer[\text{\small{IF FALSE}}]
		{
			\IF{false}{1}{0} \to 0
		}
		{}
	}
\]
\\
\[
	\APP{3}{0} \not\to
\]
To let the term evolve to a stuck one earlier the (APP 2) rule could be substituted with the following
\[
	\infer[\text{\small{APP 2'}}]
	{
		\APP{(\FN{x}{M_1})}{M_2} \to \APP{(\FN{x}{M_1})}{M_2'}
	}
	{M_2 \to M_2'}
\]
with this semantics it would take one step instead of three to reach a stuck term.
